## 1
```
T(0) = 0
T(1) = 1
T(n) = -4*T(n - 1) - 4*T(n - 2)

t^n = -4t^(n-1) -4t^(n-2)
t^n + 4t^(n-1) + 4t^(n-2) = 0
t^(n-2) (t^2 + 4t + 4) = 0
t = -2

T(n) = (a+bn)(-2)^n
a = 0
1 = (a+b)(-2)
1 = -2a - 2b
b = -1/2
T(n) = (-1/2n)(-2)^n
```

## 2 - Incomplete
```
T(0) = 2
T(1) = 1
T(n) = T(n - 1) + 2*T(n - 2) + 2

t^n = t^(n-1) + 2t^(n-2)
t^n - t^(n-1) - 2t^(n-2) = 0
t^(n-2) (t^2 - t - 2) = 0
t= -1, 2

T(n) = a(-1)^n + b(2)^n + c

2 = a + b + c
1 = -a + 2b + c
3 = 3b + c
```

## 3 - Incomplete
```
T(0) = 3
T(1) = 5
T(n) = 4*T(n - 1) - 3*T(n - 2) + n

t^n = 4t^(n-1) - 3t^(n-2)
t^n - 4t^(n-1) + 3t^(n-2) = 0
t^(n-2) (t^2 - 4t + 3) = 0
t = 1, 3

T(n) = a(1)^n + b(3)^n + cn
T(n) = a + b(3)^n + cn
3 = a + b
5 = a + 3b + c
```

## 4 - Incorrect
```
T(0) = 9
T(1) = 10
T(2) = 32
T(n) = 7*T(n - 2) + 6*T(n - 3)

t^n = 7t^(n-2) + 6t^(n-3)
t^n - 7t^(n-2) - 6t^(n-3) = 0
t^(n-3) (t^3 - 7t - 6) = 0
t = -1, -2, 3

T(n) = a(-1)^n + b(-2)^n + c(3)^n
0 = a + b + c
10 = -a - 2b + 3c
32 = a + 4b + 9c
a = -11/2
b = 12/5
c = 31/10
T(n) = (-11/2)(-1)^n + (12/5)(-2)^n + (31/10)(3)^n
```